program_logic/ectx_lifting.v
@@ -20,7 +20,7 @@ Lemma wp_lift_head_step E Φ e1 :
   to_val e1 = None →
   (|={E,∅}=> ∃ σ1, ■ head_reducible e1 σ1 ★ ▷ ownP σ1 ★
     ▷ ∀ e2 σ2 efs, ■ head_step e1 σ1 e2 σ2 efs ★ ownP σ2
-          ={∅,E}=★ WP e2 @ E {{ Φ }} ★ wp_fork efs)
+          ={∅,E}=★ WP e2 @ E {{ Φ }} ★ [★ list] ef ∈ efs, WP ef {{ _, True }})
   ⊢ WP e1 @ E {{ Φ }}.
 Proof.
   iIntros (?) "H". iApply (wp_lift_step E); try done.
@@ -33,7 +33,8 @@ Lemma wp_lift_pure_head_step E Φ e1 :
   to_val e1 = None →
   (∀ σ1, head_reducible e1 σ1) →
   (∀ σ1 e2 σ2 efs, head_step e1 σ1 e2 σ2 efs → σ1 = σ2) →
-  (▷ ∀ e2 efs σ, ■ head_step e1 σ e2 σ efs → WP e2 @ E {{ Φ }} ★ wp_fork efs)
+  (▷ ∀ e2 efs σ, ■ head_step e1 σ e2 σ efs →
+    WP e2 @ E {{ Φ }} ★ [★ list] ef ∈ efs, WP ef {{ _, True }})
   ⊢ WP e1 @ E {{ Φ }}.
 Proof.
   iIntros (???) "H". iApply wp_lift_pure_step; eauto. iNext.
@@ -44,7 +45,8 @@ Lemma wp_lift_atomic_head_step {E Φ} e1 σ1 :
   atomic e1 →
   head_reducible e1 σ1 →
   ▷ ownP σ1 ★ ▷ (∀ v2 σ2 efs,
-  ■ head_step e1 σ1 (of_val v2) σ2 efs ∧ ownP σ2 -★ (|={E}=> Φ v2) ★ wp_fork efs)
+  ■ head_step e1 σ1 (of_val v2) σ2 efs ∧ ownP σ2 -★
+    (|={E}=> Φ v2) ★ [★ list] ef ∈ efs, WP ef {{ _, True }})
   ⊢ WP e1 @ E {{ Φ }}.
 Proof.
   iIntros (??) "[? H]". iApply wp_lift_atomic_step; eauto. iFrame. iNext.
@@ -56,13 +58,36 @@ Lemma wp_lift_atomic_det_head_step {E Φ e1} σ1 v2 σ2 efs :
   head_reducible e1 σ1 →
   (∀ e2' σ2' efs', head_step e1 σ1 e2' σ2' efs' →
     σ2 = σ2' ∧ to_val e2' = Some v2 ∧ efs = efs') →
-  ▷ ownP σ1 ★ ▷ (ownP σ2 -★ (|={E}=> Φ v2) ★ wp_fork efs) ⊢ WP e1 @ E {{ Φ }}.
+  ▷ ownP σ1 ★ ▷ (ownP σ2 -★
+    (|={E}=> Φ v2) ★ [★ list] ef ∈ efs, WP ef {{ _, True }})
+  ⊢ WP e1 @ E {{ Φ }}.
 Proof. eauto using wp_lift_atomic_det_step. Qed.
+
+Lemma wp_lift_atomic_det_head_step' {E Φ e1} σ1 v2 σ2 :
+  atomic e1 →
+  head_reducible e1 σ1 →
+  (∀ e2' σ2' efs', head_step e1 σ1 e2' σ2' efs' →
+    σ2 = σ2' ∧ to_val e2' = Some v2 ∧ [] = efs') →
+  ▷ ownP σ1 ★ ▷ (ownP σ2 ={E}=★ Φ v2) ⊢ WP e1 @ E {{ Φ }}.
+Proof.
+  intros. rewrite -(wp_lift_atomic_det_head_step σ1 v2 σ2 [])
+    ?big_sepL_nil ?right_id; eauto.
+Qed.
 
 Lemma wp_lift_pure_det_head_step {E Φ} e1 e2 efs :
   to_val e1 = None →
   (∀ σ1, head_reducible e1 σ1) →
-  (∀ σ1 e2' σ2 efs', head_step e1 σ1 e2' σ2 efs' → σ1 = σ2 ∧ e2 = e2' ∧ efs = efs')→
-  ▷ (WP e2 @ E {{ Φ }} ★ wp_fork efs) ⊢ WP e1 @ E {{ Φ }}.
+  (∀ σ1 e2' σ2 efs', head_step e1 σ1 e2' σ2 efs' → σ1 = σ2 ∧ e2 = e2' ∧ efs = efs') →
+  ▷ (WP e2 @ E {{ Φ }} ★ [★ list] ef ∈ efs, WP ef {{ _, True }})
+  ⊢ WP e1 @ E {{ Φ }}.
 Proof. eauto using wp_lift_pure_det_step. Qed.
+
+Lemma wp_lift_pure_det_head_step' {E Φ} e1 e2 :
+  to_val e1 = None →
+  (∀ σ1, head_reducible e1 σ1) →
+  (∀ σ1 e2' σ2 efs', head_step e1 σ1 e2' σ2 efs' → σ1 = σ2 ∧ e2 = e2' ∧ [] = efs') →
+  ▷ WP e2 @ E {{ Φ }} ⊢ WP e1 @ E {{ Φ }}.
+Proof.
+  intros. rewrite -(wp_lift_pure_det_step e1 e2 []) ?big_sepL_nil ?right_id; eauto.
+Qed.
 End wp.
